finished first version of the Tutorial

theories/Tutorial.v
@@ -1,5 +1,22 @@
-(* Tutorial *)
+(** * Zooid Tutorial/walkthrough *)
+(** ** Introduction
 
+This file contains a walkthrough/tutorial on how to write Zooid
+specification and processes. For succinctness this tutorial assumes
+familiarity with the Coq proof assistant, the OCaml programming
+language, and the theory of multiparty session types.
+
+For the complete code, the source of this file is available in the
+Zooid distribution in the directory <<theories/Tutorial.v>>. After
+reading the HTML version of this document, we encourage you to go
+interactively over the file. This will allow you to modify and test
+things, and moreover go over the proofs step by step. <<Tutorial.v>>
+also contains extra theorems whose study would help the understanding
+of the more complex proofs.
+
+*)
+
+(* begin hide *)
 From mathcomp Require Import all_ssreflect seq.
 From mathcomp Require Import finmap.
 
@@ -19,179 +36,413 @@ Set Implicit Arguments.
 Unset Strict Implicit.
 Import Prenex Implicits.
 
-
-
 Open Scope proc_scope.
 
+(* end hide *)
 
-(*
- * PingPong Example
+(** ** The protocol definition: a global type
+
+In this tutorial we will explore a binary protocol for clarity of
+presentation. The objective is to discuss progressively more complex
+implementations to motivate how one may approach programming with
+Zooid.
+
+The Ping Pong protocol definition we use here correspond to the
+intuition of it. Let's explore it in more detail.
+*)
+
+(** First we define a pair of identifiers for the two roles, we use
+natural numbers to represent each participant. *)
+
+Definition pp_server := 0. Definition pp_client := 1.
+
+(** In this protocol, the server will wait for messages from the
+client, the client will choose to either send a 'Ping' message and
+wait for the 'Pong' response, and repeat, or it will choose to send
+'Bye' to end the protocol.
+
+For this purpose we define three message identifiers as labels of each
+message. Again, labels are also reprsented by natural numbers.
  *)
 
-Definition Bye := 0.
-Definition Ping := 1.
-Definition Pong := 1.
 
-Definition pp_server := 0.
-Definition pp_client := 1.
+Definition Bye := 0. Definition Ping := 1. Definition Pong := 1.
+
+(**
+
+At this point we are ready to specify the global type, we do explore
+in a step by step manner, and provide the full global type in the end.
+
+
+This protocol is recursive, and it repeats itself from the begining,
+so the first constructor is [g_rec] insicating that the fix point
+starts here.
+
+[Definition ping_pong := g_rec ...]
+
+
+Then the client has the choice of finishing the interaction or
+requesting a ping. The constructor [g_msg] allows one to express this,
+it takes the source and target of the message and a list of messages
+and their payload type and continuations. In this case we leave the
+continuations as ellipsis for now. The payload for the message [Bye]
+is just unit since the interaction has finished and no more
+information is required and the payload for [Ping] is a natural number
+for the server.
+
+[Definition ping_pong := g_rec (g_msg pp_client pp_server [:: (Bye,
+  (T_unit, ...) (Ping, (T_nat, ...))]])]
+
+When the client sends the [Bye] label then the continuation is simply
+to end ([g_end]):
+
+[Definition ping_pong := g_rec ( g_msg pp_client pp_server [:: (Bye,
+  (T_unit, g_end)); (Ping, (T_nat, ... ).]])]
+
+On the case of the [Ping] label the behaviour is to let the server
+respond with the [Pong] label and another natural number [ g_msg
+pp_server pp_client [:: (Pong, (T_nat, ...))])) ]]
+
+So far our still incomplete definition looks like this:
+
+[Definition ping_pong := g_rec ( g_msg pp_client pp_server [:: (Bye,
+  (T_unit, g_end)); (Ping, (T_nat, g_msg pp_server pp_client [::
+  (Pong, (T_nat, ...))])) ] ).]])]
+
+After the [Pong] label, both the client and the server are ready to do
+another run of the protocol. Zooid uses de-Bruijn indices for its
+recursion variables (introduced by the [g_rec] constructor). Since
+there is only one recursion constructor, we invke it with [g_var 0].
+
+With this we have completely specified the communication protocol for
+this example.
+
+The global type for this protocol is:
+ *)
 
 Definition ping_pong :=
-  g_rec (
-      g_msg pp_client pp_server
-            [::
-               (Bye, (T_unit, g_end));
-               (Ping,
-                (T_nat,
-                 g_msg pp_server pp_client [:: (Pong, (T_nat, g_var 0))]))
-            ]
-    ).
+  g_rec ( g_msg pp_client pp_server
+    [:: (Bye,  (T_unit, g_end));
+        (Ping, (T_nat, g_msg pp_server pp_client
+          [:: (Pong, (T_nat, g_var 0))]))]).
+
+
+(**
+
+Note: the global type specifies all the acceptable behaviours by the
+client and server, yet implementations get to choose which labels to
+send, and the policies regarding the payloads (in this case the
+numbers sent back and forth in the ping pongs.
+
+----
+*)
+
+(** ** The local types of the participants
+
+The local types for each participants are derived automatically by the
+certified implementations.
+
+*)
+
 
 Definition pp_env := \project ping_pong.
 Definition pp_server_lt := \get pp_env pp_server.
 Definition pp_client_lt := \get pp_env pp_client.
 
-Definition ping_pong_server : wt_proc pp_server_lt :=
-     loop (
-       \branch pp_client
-        [alts
-        | \lbl Bye, _ : T_unit;
-            finish
-        | \lbl Ping, x : T_nat;
-            (\send pp_client Pong x (jump 0))
-        ]
-     ).
+(** [pp_env] contains the types for all participants from which we get
+the types of each role.
 
+----*)
+
+
+(** ** The process implementations
+
+*** The implementation of the server
+
+First, we will implement the server. The server is in a sense simpler
+because it will implement all the behaviours since in this protocol
+only the client has meaningful choices (i.e.: to ping or quit). As a
+policy for the payloads this server will simple echo back the payload
+of the [Ping] message.
+
+First start with a definition of an intrinsically typed process
+[wt_proc] of type [pp_server_lt].
+
+[Definition ping_pong_server : wt_proc pp_server_lt :=..]
+
+The protocol starts with a fix point, so the first (smart) constructor
+should be [loop] to allow for the recursion to happen.
+
+[Definition ping_pong_server : wt_proc pp_server_lt := loop ..]
+
+Following the protocol, the server has to respond to the client's
+choice, we do this with [\branch pp_client [alts | ... ]] where the
+alternatives are either [Bye] carrying a unit or [Ping] carrying a
+natural number: [ [alts | \lbl Bye, _ : T_unit; ... | \lbl Ping, x :
+T_nat; ...] ]
+
+The server quits if it receives [Bye] with the process smart
+constructor [finish] and otherwise it sends back [Pong] with the same
+value it received in variable [x].
+
+[\send pp_client Pong x ...]
+
+To repeat the loop, we use again de-bruijn indices and we jump back
+with [jump 0].
+
+The complete definition of the server is thus:
+ *)
+
+Definition ping_pong_server : wt_proc pp_server_lt :=
+  loop ( \branch pp_client
+         [alts | \lbl Bye, _ : T_unit; finish
+               | \lbl Ping, x : T_nat; (\send pp_client Pong x (jump 0))] ).
+
+(* begin hide *)
+
+(* this definition simple projects the untyped term from the
+intrinsically typed process *)
 
 Definition to_proc p := get_proc (projT2 p).
 
+(* This lemma is just to show that the untyped process also admits the
+global type *)
 Lemma pp_s1 : of_lt_unr pp_server (get_proc ping_pong_server) pp_env.
-Proof.
-  exists pp_server_lt;split=>//.
-  apply: (projT2 ping_pong_server).
-  by apply: l_expand_unr.
-Qed.
+Proof. exists pp_server_lt;split=>//. apply: (projT2
+ping_pong_server). by apply: l_expand_unr. Qed.
 
+(* end hide *)
+
+
+(** *** The first client -- Always be saying goodbye
+
+This first client is the simplest possible one. I just always asks the
+server to finish the interaction by sending [Bye].
+
+*)
 
 Definition ping_pong_client0 : wt_proc pp_client_lt :=
-     loop (
-       \select pp_server
-        [sel
-        | \otherwise => Bye, tt \as T_unit ! finish
-        | \skip => Ping, T_nat ! l_msg l_recv pp_server [:: (Pong, (T_nat, l_var 0))]
+  loop (\select pp_server
+         [sel | \otherwise => Bye, tt \as T_unit ! finish
+              | \skip => Ping, T_nat !
+                l_msg l_recv pp_server [:: (Pong, (T_nat, l_var 0))]
+         ]).
 
-        ]
-     ).
+(** In this client we use the [\select pp_server ...] construct to
+make a choice, for this we need to offer a series of conditions that
+if met they are executed, or skipping some parts of the protocol. The
+skips are necessary to simplify arguing that the local type of the
+process corresponds to the one inferred from the terms (i.e.: avoiding
+this would lead to more proof obligations).
 
+The selection arguments:
+[ [sel | \otherwise => Bye, tt \as T_unit !...| \skip => Ping, T_nat !...] ]
+has two branches [\otherwise] that is
+always taken and [\skip] that says that this branch is never taken,
+note that [\skip] is annotated with the type of the continuation that
+is skipped.
+ *)
 
+(* begin hide *)
 Lemma pp_c0 : of_lt_unr pp_client (get_proc ping_pong_client0) pp_env.
 Proof.
-  exists pp_client_lt; split.
-  - by apply: (projT2 ping_pong_client0).
-  - by apply: l_expand_unr.
+exists pp_client_lt; split.
+- by apply: (projT2 ping_pong_client0).
+- by apply: l_expand_unr.
 Qed.
+(* end hide *)
+
+(** *** The second client -- Always be pinging
+
+This client is more interesting than the previous one, by always
+choosing to ping and never terminating.
+
+*)
 
 Definition ping_pong_client1 : wt_proc pp_client_lt :=
-     loop (
-       \select pp_server
-        [sel
-        | \skip      => Bye , T_unit ! l_end
-        | \otherwise => Ping, 1 \as T_nat !
-              (\recv pp_server \lbl Pong, x : T_nat; (jump 0))
-        ]
-     ).
+  loop ( \select pp_server
+         [sel | \skip => Bye , T_unit ! l_end
+              | \otherwise => Ping, 1 \as T_nat !
+                (\recv pp_server \lbl Pong, x : T_nat; (jump 0)) ] ).
 
+(** The implementation of this client does not use new elements, it
+simply uses the elements that we knew of in a different way. *)
+
+(* begin hide *)
 Lemma pp_c1 : of_lt_unr pp_client (get_proc ping_pong_client1) pp_env.
 Proof.
-  exists pp_client_lt; split.
-  - by apply: (projT2 ping_pong_client1).
-  - by apply: l_expand_unr.
+exists pp_client_lt; split.
+- by apply: (projT2 ping_pong_client1).
+- by apply: l_expand_unr.
 Qed.
+(* end hide *)
+
+
+
+(** *** The third client -- Always be pinging just one time
+
+This client behaves by sending one ping and then terminating. Also,
+until now, all the clients followed the structure of the type step by
+step. What we mean, is that they all do first the [loop], and then
+[\select], and so and so. In this case, since we only want to send one
+[Ping] and then terminate with [Bye] we have avoided the [loop]
+construct.
+
+Here is the definition of the process:
+*)
 
 Definition ping_pong_client2 :=
-  [proc
-     \select pp_server
-     [sel
-     | \otherwise => Bye, tt \as T_unit ! finish
-     | \skip => Ping, T_nat !
-             l_msg l_recv pp_server
-             [:: (Pong, (T_nat, pp_client_lt))]
-     ]
-  ].
+  [proc \select pp_server
+        [sel | \otherwise => Bye, tt \as T_unit ! finish
+             | \skip => Ping, T_nat !
+               l_msg l_recv pp_server [:: (Pong, (T_nat, pp_client_lt))] ] ].
 
+(**
+
+Things to notice:
+
+- no type annotation, we use Coq's type inference to get the type of
+  this Zooid program.
+
+- instead of starting with [loop] we start the process with [[proc
+  ...]] to signal to Coq that this is a Zooid implicitely typed
+  process.
+
+- instead of sending [Bye] after receiving [Pong] we call
+  [pp_client_lt] (the process that always says bye) to terminate the
+  execution of the protocol and not have to implement it again.
+
+This implementation strategy is more versatile, allowing us to write
+process that are not structurally folloing their type's shape.
+However, the inferred type is not 'obviously' the same as expected,
+because of some unfoldings. In order to fill that gap the following
+lemma fills that gap by showing that the process admits the right type
+([to_proc] extracts the untyped process from the intrinsically typed
+one).
+*)
 
 Lemma pp_c2 : of_lt_unr pp_client (to_proc ping_pong_client2) pp_env.
 Proof.
   exists (projT1 ping_pong_client2); split.
   - by apply: (projT2 (projT2 ping_pong_client2)).
   - rewrite -[projT1 ping_pong_client2]/(lunroll 1 pp_client_lt).
-    by rewrite -LUnroll_ind; apply: l_expand_unr.
+      by rewrite -LUnroll_ind;
+      apply: l_expand_unr.
 Qed.
 
+(** The proof should be simple enough as it resorts unroll and unravel
+the coinductive types. *)
+
+
+(** *** The fourth client -- Always be useful
+
+This client shows how to use Coq infrastructure in Zooid code taking
+advantage of Zooid's nature a shallow embedding in Coq.
+
+This version of the client is the n-ary version of the previous one,
+and we compute that using Coq's [Fixpoint]
+
+The first definition is a recursive function that computes the process
+that sends [n] times [Ping]. *)
 
 Fixpoint ping_pong_client3 n {struct n}:=
   match n with
-  | 0 =>
-    [proc \select pp_server
-          [sel
-          | \otherwise => Bye, tt \as T_unit ! finish
-          | \skip => Ping, T_nat !
-                                 l_msg l_recv pp_server
-                                 [:: (Pong, (T_nat, pp_client_lt))]]
-    ]
-  | m.+1 =>
-    [proc \select pp_server
-          [sel
-          | \skip => Bye, T_unit ! l_end
-          | \otherwise =>
-            Ping, n \as T_nat !
-              (\recv pp_server \lbl Pong, x : T_nat; projT2 (ping_pong_client3 m))
-          ]
-    ]
+  | 0 => [proc
+            \select pp_server
+            [sel | \otherwise => Bye, tt \as T_unit ! finish
+             | \skip => Ping, T_nat !
+                        l_msg l_recv pp_server
+                          [:: (Pong, (T_nat, pp_client_lt))]] ]
+  | m.+1 => [proc
+               \select pp_server
+               [sel | \skip =>
+  Bye, T_unit ! l_end | \otherwise => Ping, n \as T_nat ! (\recv
+  pp_server \lbl Pong, x : T_nat; projT2 (ping_pong_client3 m)) ] ]
   end.
 
+(** This unravels the local type n times. *)
 Fixpoint l_unravel_n n L :=
   match n, lunroll (lrec_depth L) L with
   | n.+1, l_msg p q Ks => l_msg p q [seq (K.1, (K.2.1, l_unravel_n n K.2.2)) | K <- Ks]
-  | _, _ => L
-  end.
+  | _, _ => L end.
 
+
+(** This shows that it works for one unravelling. The general proof is
+left as an excercise. *)
 Goal projT1 (ping_pong_client3 0) = l_unravel_n 1 pp_client_lt.
     by [].
 Qed.
 
+(** *** The fifth client -- Always be willing to stop
+
+This version of the process sends [Ping] until the [Pong] payload is
+larger than 3.
+
+The only new construct in this client is the the [\case] clause in
+[\select] that allows for a condition to be specified to continue with
+this branch or continue with the rest.
+
+Spend some time convincing yourself that the implementatio behaves
+like the previous description.
+
+*)
+
 
 Definition ping_pong_client4 :=
   [proc \select pp_server
-        [sel
-        | \skip => Bye, T_unit ! l_end
-        | \otherwise => Ping, 1 \as T_nat !
-              loop(
-                \recv pp_server \lbl Pong, x : T_nat;
-                  \select pp_server
-                   [sel
-                   | \case (x > 3) => Bye, tt \as T_unit ! finish
-                   | \otherwise => Ping, x + 1 \as T_nat ! jump 0
-                   ]
-              )
-        ]
-  ].
-Definition ppc4_t1 := Eval compute in projT1 ping_pong_client4.
-Definition ppc4_t2 := Eval compute in get_proc (projT2 ping_pong_client4).
+        [sel | \skip => Bye, T_unit ! l_end
+         | \otherwise => Ping, 1 \as T_nat !
+           loop(\recv pp_server \lbl Pong, x : T_nat;
+               \select pp_server
+                [sel | \case (x > 3) => Bye, tt \as T_unit ! finish
+                     | \otherwise => Ping, x + 1 \as T_nat ! jump 0])]].
 
+
+(** By now you have read [ping_pong_client4] and you may be convinced
+that it follows the protocol. However, given that the process is not
+constructed to follow the exact structure of the local type, Coq is
+also not convinced.
+
+The following theorem shows that the inferred type [projT1
+ping_pong_client4 ] and [pp_client_lt] are unrollings of eachother.
+*)
 Goal forall Li Lc, (Li = projT1 ping_pong_client4 /\
-                    Lc = l_expand pp_client_lt) ->
-                   LUnroll Li Lc.
+                    Lc = l_expand pp_client_lt) -> LUnroll Li Lc.
+Proof.
   apply/paco2_acc=> r _ /(_ _ _ (conj erefl erefl))/=-CIH Li Lr [->->].
-  apply: paco2_fold; rewrite l_expand_once/=; constructor=>/=;
-    first by apply/same_dom_eta/same_dom_extend/same_dom_extend/same_dom_refl.
+  apply: paco2_fold;
+    rewrite l_expand_once/=; constructor=>/=; first by
+      apply/same_dom_eta/same_dom_extend/same_dom_extend/same_dom_refl.
   move=> l Ty G G'; rewrite /extend/empty/=.
-  case: ifP=>//;
-    first by move=>_ [<-<-] [<-]; left; apply/paco2_fold;
-             rewrite l_expand_once; constructor.
+  case:
+    ifP=>//; first by move=>_ [<-<-] [<-]; left;
+      apply/paco2_fold; rewrite l_expand_once; constructor.
   case: ifP=>//; move=> _ _ [<-<-] [<-]; left; apply/paco2_fold.
   constructor=>/=; left; rewrite l_expand_once/=.
-  apply: paco2_fold; constructor;
-    first by apply/same_dom_eta/same_dom_extend/same_dom_refl.
-  move=> {}l {}Ty {}G {}G'/=; rewrite /extend/empty/=.
-  by case: ifP=>// _ [<-<-] [<-]; right; apply/CIH.
+  apply: paco2_fold; constructor; first by
+      apply/same_dom_eta/same_dom_extend/same_dom_refl.
+  move=> {}l {}Ty {}G {}G'/=; rewrite
+           /extend/empty/=.
+    by case: ifP=>// _ [<-<-] [<-];
+      right; apply/CIH.
 Qed.
+
+(** This proof is also about unfoling and aligning the two types, and
+while it is a bit frutrating to do, it does not require great
+insights. In the future, Zooid will provide tools to automate these
+proofs as much as possible.
+
+---- ** Final words
+
+This tutorial explores how to implement processes using Zooid. The
+remaining aspects are how to extract the code, and for that we invite
+you to check the <<theories/Code.v>> file where all the examples are
+extracted. Finally, to connect to the OCaml, first use the interactive
+example walkthrough by running <./run.sh> from the root directory of
+the Zooid distribution/docker container that contains pointers and
+explanation of all the important details.
+
+_Thank you very much_ for your attention.
+
+The Zooid team.
+*)
